theories/L6_PCPS/shrink_proto.v
@@ -1,0 +1,640 @@
+Require Import Coq.Strings.String.
+Require Import Coq.Sets.Ensembles Coq.ZArith.ZArith.
+Require Import L6.Ensembles_util L6.map_util L6.List_util.
+Require Import L6.state L6.alpha_conv L6.identifiers L6.functions L6.shrink_cps.
+Require Import L6.Prototype.
+Require Import L6.cps_proto L6.proto_util.
+
+Require Import Lia.
+
+Require Import Coq.Lists.List.
+Import ListNotations.
+
+Unset Strict Unquote Universe Mode.
+
+(** * Shrink rewrites *)
+
+(* Known functions *)
+
+(* The function definition f(xs) = e_body (with fun tag ft) is known at C⟦e⟧ if
+   f was defined in an earlier bundle.
+   (Contrast this with the definition for inlining, which also allows inlining of
+    functions within the same bundle) *)
+Definition known_function {A} (f : var) (ft : fun_tag) (xs : list var) (e_body : exp)
+          (C : exp_c A exp_univ_exp) : Prop :=
+  (exists D fds E, C = D >:: Efun1 fds >++ E /\ List.In (Ffun f ft xs e_body) fds).
+
+(* Known constructor values *)
+
+(* (x ↦ Con c ys) ∈ C *)
+Definition known_ctor {A} x c ys (C : exp_c A exp_univ_exp) : Prop :=
+  exists D E, C = D >:: Econstr3 x c ys >++ E.
+
+(* Occurrence counts *)
+
+Definition count_var (x_in x : var) : nat := if (![x_in] =? ![x])%positive then 1 else 0.
+Definition total : list nat -> nat := fold_right plus 0.
+Definition count_vars x_in (xs : list var) : nat := total (map (count_var x_in) xs).
+Definition count_ces' (count_exp : var -> exp -> nat) x_in (ces : list (ctor_tag * _)) : nat :=
+  total (map (fun '(_, e) => count_exp x_in e) ces).
+Definition count_fds' (count_exp : var -> exp -> nat) x_in (fds : list fundef) : nat :=
+  total (map (fun '(Ffun _ _ _ e) => count_exp x_in e) fds).
+Fixpoint count_exp x_in e {struct e} : nat :=
+  match e with
+  | Econstr x c ys e => count_vars x_in ys + count_exp x_in e
+  | Ecase x ces => count_var x_in x + count_ces' count_exp x_in ces
+  | Eproj x c n y e => count_var x_in y + count_exp x_in e
+  | Eletapp x f ft ys e => count_var x_in f + count_vars x_in ys + count_exp x_in e
+  | Efun fds e => count_fds' count_exp x_in fds + count_exp x_in e
+  | Eapp f ft xs => count_var x_in f + count_vars x_in xs
+  | Eprim x p ys e => count_vars x_in ys + count_exp x_in e
+  | Ehalt x => count_var x_in x
+  end.
+Definition count_ces := count_ces' count_exp.
+Definition count_fds := count_fds' count_exp.
+
+Inductive shrink_step : exp -> exp -> Prop :=
+(* Case folding *)
+| shrink_cfold : forall (C : frames_t exp_univ_exp _) x c ys e ces,
+  known_ctor x c ys C /\ In (c, e) ces ->
+  shrink_step (C ⟦ Ecase x ces ⟧) (C ⟦ Rec e ⟧)
+(* Projection folding *)
+| shrink_pfold : forall (C : frames_t exp_univ_exp _) x c ys y y' t n e,
+  known_ctor x c ys C /\ nthN ys n = Some y' ->
+  shrink_step (C ⟦ Eproj y t n x e ⟧) (C ⟦ Rec (rename_all' (M.set ![y] ![y'] (M.empty _)) e) ⟧)
+(* Dead variable elimination *)
+| shrink_dead_constr1 : forall (C : frames_t exp_univ_exp exp_univ_exp) x c ys e,
+  ~ ![x] \in occurs_free ![e] ->
+  shrink_step (C ⟦ Econstr x c ys e ⟧) (C ⟦ Rec e ⟧)
+| shrink_dead_constr2 : forall (C : frames_t exp_univ_exp exp_univ_exp) x c ys e,
+  ~ ![x] \in occurs_free ![e] ->
+  BottomUp (shrink_step (C ⟦ Econstr x c ys e ⟧) (C ⟦ e ⟧))
+| shrink_dead_proj1 : forall (C : frames_t exp_univ_exp exp_univ_exp) x t n y e,
+  ~ ![x] \in occurs_free ![e] ->
+  shrink_step (C ⟦ Eproj x t n y e ⟧) (C ⟦ Rec e ⟧)
+| shrink_dead_proj2 : forall (C : frames_t exp_univ_exp exp_univ_exp) x t n y e,
+  ~ ![x] \in occurs_free ![e] ->
+  BottomUp (shrink_step (C ⟦ Eproj x t n y e ⟧) (C ⟦ e ⟧))
+| shrink_dead_prim1 : forall (C : frames_t exp_univ_exp exp_univ_exp) x p ys e,
+  ~ ![x] \in occurs_free ![e] ->
+  shrink_step (C ⟦ Eprim x p ys e ⟧) (C ⟦ Rec e ⟧)
+| shrink_dead_prim2 : forall (C : frames_t exp_univ_exp exp_univ_exp) x p ys e,
+  ~ ![x] \in occurs_free ![e] ->
+  BottomUp (shrink_step (C ⟦ Eprim x p ys e ⟧) (C ⟦ e ⟧))
+| shrink_dead_fun1 : forall (C : frames_t exp_univ_list_fundef exp_univ_exp) f ft xs e fds,
+  count_exp f (C ⟦ Ffun f ft xs e :: fds ⟧) = 0 ->
+  shrink_step (C ⟦ Ffun f ft xs e :: fds ⟧) (C ⟦ Rec fds ⟧)
+| shrink_dead_fun2 : forall (C : frames_t exp_univ_list_fundef exp_univ_exp) f ft xs e fds,
+  count_exp f (C ⟦ Ffun f ft xs e :: fds ⟧) = 0 ->
+  BottomUp (shrink_step (C ⟦ Ffun f ft xs e :: fds ⟧) (C ⟦ fds ⟧))
+| shrink_dead_funs : forall (C : frames_t exp_univ_exp exp_univ_exp) e,
+  BottomUp (shrink_step (C ⟦ Efun [] e ⟧) (C ⟦ e ⟧))
+(* Inlining *)
+| shrink_inline : forall (C : frames_t exp_univ_exp exp_univ_exp) f ft ft' xs ys e σ,
+  known_function f ft' xs e C /\
+  count_exp f (C ⟦ Eapp f ft ys ⟧) = 1 ->
+  set_lists ![xs] ![ys] (M.empty _) = Some σ ->
+  shrink_step (C ⟦ Eapp f ft ys ⟧) (C ⟦ Rec (rename_all' σ e) ⟧).
+
+(** * Known functions *)
+
+Definition R_fns {A} (C : exp_c A exp_univ_exp) : Set := {
+  ρ : fun_map |
+  forall f ft xs e_body, M.get ![f] ρ = Some (ft, xs, e_body) ->
+  known_function f ft xs e_body C }.
+
+Instance Preserves_R_fns : Preserves_R _ exp_univ_exp (@R_fns).
+Proof.
+  intros A B fs f [ρ Hρ]; destruct f; lazymatch goal with
+  | |- R_fns (fs >:: Efun1 ?fds') => rename fds' into fds
+  | _ =>
+    exists ρ; intros f' ft' xs' e_body' Hget'; specialize (Hρ f' ft' xs' e_body' Hget');
+    destruct Hρ as [D [fds [E [Hctx Hin]]]];
+    match goal with |- known_function _ _ _ _ (_ >:: ?f) => exists D, fds, (E >:: f); now subst fs end
+  end.
+  exists (add_fundefs fds ρ); intros [f] ft xs e_body Hget; cbn in *.
+  apply add_fundefs_Some in Hget; destruct Hget as [|Hnotin]; [now exists fs, fds, <[]>|].
+  specialize (Hρ (mk_var f) ft xs e_body Hnotin); destruct Hρ as [D [fds' [E [Hctx Hin]]]].
+  exists D, fds', (E >:: Efun1 fds); now subst fs.
+Defined.
+
+(** * Known constructors *)
+
+Definition ctx_map := M.tree (ctor_tag * list var).
+Definition R_ctors {A} (C : exp_c A exp_univ_exp) : Set := {
+  ρ : ctx_map |
+  forall x c ys, M.get ![x] ρ = Some (c, ys) -> known_ctor x c ys C }.
+
+Instance Preserves_R_ctors : Preserves_R _ exp_univ_exp (@R_ctors).
+Proof.
+  intros A B fs f [ρ Hρ]; destruct f; lazymatch goal with
+  | |- R_ctors (fs >:: Econstr3 ?x' ?c' ?ys') => rename x' into x, c' into c, ys' into ys
+  | _ =>
+    exists ρ; intros x' c' ys' Hget'; specialize (Hρ x' c' ys' Hget');
+    destruct Hρ as [D [E Hctx]];
+    match goal with |- known_ctor _ _ _ (_ >:: ?f) => exists D, (E >:: f); now subst fs end
+  end.
+  destruct x as [x]; exists (M.set x (c, ys) ρ); intros [x'] c' ys' Hget'; cbn in *.
+  destruct (Pos.eq_dec x' x); [subst; rewrite M.gss in Hget'; inv Hget'; now exists fs, <[]>|].
+  rewrite M.gso in Hget' by auto; destruct (Hρ (mk_var x') c' ys' Hget') as [D [E Hctx]].
+  exists D, (E >:: Econstr3 (mk_var x) c ys); now subst fs.
+Defined.
+
+(** * Occurrence counts *)
+
+Definition c_map : Set := M.tree positive.
+
+Definition census_var (x : var) (δ : c_map) : c_map :=
+  let x := ![x] in
+  match M.get x δ with
+  | Some n => M.set x (n + 1)%positive δ
+  | None => M.set x 1%positive δ
+  end.
+Definition census_list {A} (census : A -> c_map -> c_map) (xs : list A) (δ : c_map) :=
+  fold_right census δ xs.
+Definition census_vars := census_list census_var.
+Definition census_ces' (census_exp : exp -> c_map -> c_map) : list (ctor_tag * _) -> _ -> _ :=
+  census_list (fun '(c, e) δ => census_exp e δ).
+Definition census_fds' (census_exp : exp -> c_map -> c_map) :=
+  census_list (fun '(Ffun f ft xs e) δ => census_exp e δ).
+Fixpoint census_exp (e : exp) (δ : c_map) {struct e} : c_map :=
+  match e with
+  | Econstr x c ys e => census_vars ys (census_exp e δ)
+  | Ecase x ces => census_var x (census_ces' census_exp ces δ)
+  | Eproj x c n y e => census_var y (census_exp e δ)
+  | Eletapp x f ft ys e => census_var f (census_vars ys (census_exp e δ))
+  | Efun fds e => census_fds' census_exp fds (census_exp e δ)
+  | Eapp f ft xs => census_var f (census_vars xs δ)
+  | Eprim x p ys e => census_vars ys (census_exp e δ)
+  | Ehalt x => census_var x δ
+  end.
+Definition census_ces := census_ces' census_exp.
+Definition census_fds := census_fds' census_exp.
+
+(* [census] computes occurrence counts *)
+
+Definition census_count (x : var) δ :=
+  match M.get ![x] δ with
+  | Some n => Pos.to_nat n
+  | None => 0
+  end.
+
+Lemma census_var_corresp x_in x n δ δ' :
+  δ' = census_var x_in δ ->
+  census_count x δ = n ->
+  census_count x δ' = n + count_var x x_in.
+Proof.
+  intros Hmk Hold; unbox_newtypes; unfold census_count, census_var, count_var in *; cbn in *.
+  destruct (Pos.eqb_spec x x_in).
+  - subst. destruct (M.get x_in δ); rewrite M.gss; zify; lia.
+  - destruct (M.get x_in δ); subst; rewrite M.gso by auto; destruct (M.get x δ); zify; lia.
+Qed.
+
+Fixpoint census_vars_corresp xs x n δ δ' :
+  δ' = census_vars xs δ ->
+  census_count x δ = n ->
+  census_count x δ' = n + count_vars x xs.
+Proof.
+  destruct xs as [|x' xs].
+  - inversion 1; subst; cbn; zify; lia.
+  - cbn.
+    change (fold_right census_var δ xs) with (census_vars xs δ).
+    change (total (map (count_var x) xs)) with (count_vars x xs).
+    remember (census_vars xs δ) as δ'' eqn:Hδ''.
+    intros Hδ' Hx.
+    specialize (census_vars_corresp xs x n δ δ'' Hδ'' Hx).
+    eapply census_var_corresp in Hδ'; eauto; lia.
+Qed.
+
+Ltac collapse_primes :=
+  change (count_ces' count_exp) with count_ces in *;
+  change (count_fds' count_exp) with count_fds in *;
+  change (census_ces' census_exp) with census_ces in *;
+  change (census_fds' census_exp) with census_fds in *;
+  (* TODO: move to proto_util? *)
+  change (ces_of_proto' exp_of_proto) with ces_of_proto in *;
+  change (fundefs_of_proto' exp_of_proto) with fundefs_of_proto in *.
+
+Fixpoint census_exp_corresp' x n e δ δ' {struct e} :
+  δ' = census_exp e δ ->
+  census_count x δ = n ->
+  census_count x δ' = n + count_exp x e.
+Proof.
+  destruct e; cbn; collapse_primes; try solve [
+    remember (census_exp e δ) as δ0 eqn:Hδ0;
+    intros Hδ' Hn; specialize (census_exp_corresp' x n e δ δ0 Hδ0 Hn);
+    (eapply census_vars_corresp in Hδ' + eapply census_var_corresp in Hδ');
+    eauto; lia]. Guarded.
+  - remember (census_ces ces δ) as δ0 eqn:Hδ0; intros Hδ' Hn.
+    enough (Hces : forall x n δ δ',
+             δ' = census_ces ces δ ->
+             census_count x δ = n ->
+             census_count x δ' = n + count_ces x ces).
+    { specialize (Hces x n δ δ0 Hδ0 Hn); eapply census_var_corresp in Hδ'; eauto; lia. }
+    clear - census_exp_corresp'.
+    induction ces as [|[c e] ces IHces]; [intros; cbn in *; subst; lia|cbn].
+    intros x n δ δ' Hδ' Hn.
+    change (fold_right _ _ _) with (census_ces ces δ) in *|-.
+    change (total _) with (count_ces x ces).
+    remember (census_ces ces δ) as δ0 eqn:Hδ0.
+    eapply IHces in Hδ0; eauto.
+    eapply census_exp_corresp' in Hδ'; eauto; lia. Guarded.
+  - remember (census_exp e δ) as δ0 eqn:Hδ0.
+    intros Hδ' Hn; specialize (census_exp_corresp' x n e δ δ0 Hδ0 Hn).
+    remember (census_vars ys δ0) as δ1 eqn:Hδ1.
+    eapply census_vars_corresp in Hδ1; eauto.
+    eapply census_var_corresp in Hδ'; eauto; lia.
+  - remember (census_exp e δ) as δ0 eqn:Hδ0; intros Hδ' Hn.
+    enough (Hfds : forall x n δ δ',
+             δ' = census_fds fds δ ->
+             census_count x δ = n ->
+             census_count x δ' = n + count_fds x fds).
+    { eapply census_exp_corresp' in Hδ0; eauto; specialize (Hfds x _ δ0 δ' Hδ' Hδ0); lia. }
+    clear - census_exp_corresp'.
+    induction fds as [|[f ft xs e] fds IHfds]; [intros; cbn in *; subst; lia|cbn].
+    intros x n δ δ' Hδ' Hn.
+    change (fold_right _ _ _) with (census_fds fds δ) in *|-.
+    change (total _) with (count_fds x fds).
+    remember (census_fds fds δ) as δ0 eqn:Hδ0.
+    eapply IHfds in Hδ0; eauto.
+    eapply census_exp_corresp' in Hδ'; eauto; lia. Guarded.
+  - remember (census_vars xs δ) as δ0 eqn:Hδ0; intros Hδ' Hn.
+    eapply census_vars_corresp in Hδ0; eauto.
+    eapply census_var_corresp in Hδ'; eauto; lia.
+  - intros Hδ' Hn; eapply census_var_corresp in Hδ'; eauto; lia.
+Qed.
+
+Corollary census_exp_corresp e δ :
+  δ = census_exp e (M.empty _) ->
+  forall x, census_count x δ = count_exp x e.
+Proof.
+  intros Hδ x; change (count_exp x e) with (0 + count_exp x e).
+  eapply census_exp_corresp'; eauto; unfold census_count; unbox_newtypes; cbn; now rewrite M.gempty.
+Qed.
+
+(* Count = 0 --> dead variable *)
+
+Lemma plus_zero_and n m : n + m = 0 -> n = 0 /\ m = 0. Proof. lia. Qed.
+
+Lemma not_In_Setminus' {A} (S1 S2 : Ensemble A) x : ~ x \in S1 -> ~ x \in (S1 \\ S2).
+Proof. rewrite not_In_Setminus; tauto. Qed.
+
+Lemma count_dead_var x y : count_var x y = 0 -> ~ ![x] \in [set ![y]].
+Proof.
+  unbox_newtypes; unfold count_var; cbn; destruct (Pos.eqb_spec x y); inversion 1; now inversion 1.
+Qed.
+
+Fixpoint count_dead_vars x xs :
+  count_vars x xs = 0 -> ~ ![x] \in FromList ![xs].
+Proof.
+  destruct xs as [|x' xs]; [intros; inversion 1|unbox_newtypes; cbn in *].
+  change (total _) with (count_vars (mk_var x) xs).
+  intros H; apply plus_zero_and in H; destruct H as [Hx Hxs].
+  intros [Heq|Hin]; [subst; unfold count_var in Hx; now rewrite Pos.eqb_refl in Hx|].
+  now apply (count_dead_vars (mk_var x) xs Hxs).
+Qed.
+
+Fixpoint count_dead_exp x e :
+  count_exp x e = 0 -> ~ ![x] \in occurs_free ![e].
+Proof.
+  destruct e; unbox_newtypes; cbn in *; collapse_primes; repeat normalize_occurs_free; intros H;
+    repeat match goal with
+    | H : _ + _ = 0 |- _ => apply plus_zero_and in H; destruct H
+    | H : count_var _ _ = 0 |- _ => apply count_dead_var in H; cbn in *
+    | H : count_vars _ _ = 0 |- _ => apply count_dead_vars in H; cbn in *
+    | H : count_exp ?x ?e = 0 |- _ => apply (count_dead_exp x e) in H; cbn in *
+    | |- ~ _ \in (_ :|: _) => rewrite Union_demorgan; split
+    | |- ~ x \in (_ \\ _) => apply not_In_Setminus'
+    end; auto.
+  - induction ces as [|[[c] e] ces IHces]; cbn; [inversion 1; subst; now contradiction H|].
+    change (total _) with (count_ces (mk_var x) ces); normalize_occurs_free; rewrite !Union_demorgan.
+    rename H0 into Hcount; cbn in Hcount; change (total _) with (count_ces (mk_var x) ces) in Hcount.
+    apply plus_zero_and in Hcount; destruct Hcount as [He Hces]; split; [|split]; auto.
+    now apply count_dead_exp in He. Guarded.
+  - induction fds as [|[[f] [ft] xs e_body] fds IHfds]; cbn; [inversion 1; subst; now contradiction H|].
+    change (total _) with (count_fds (mk_var x) fds); normalize_occurs_free; rewrite !Union_demorgan.
+    rename H into Hcount; cbn in Hcount; change (total _) with (count_fds (mk_var x) fds) in Hcount.
+    apply plus_zero_and in Hcount; destruct Hcount as [He Hfds]; split; apply not_In_Setminus'; auto.
+    now apply count_dead_exp in He. Guarded.
+Qed.
+
+(** * Shrink inlined functions *)
+
+Definition b_map := M.tree bool.
+
+Check getd.
+Definition drop_fns_ces' (drop_fns : b_map -> exp -> exp) θ (ces : list (ctor_tag * exp)) :=
+  map (fun '(c, e) => (c, drop_fns θ e)) ces.
+Definition drop_fns_fds' (drop_fns : b_map -> exp -> exp) θ fds :=
+  fold_right
+    (fun '(Ffun f ft xs e) fds =>
+      if getd false ![f] θ
+      then Ffun f ft xs (drop_fns θ e) :: fds
+      else fds)
+    [] fds.
+Fixpoint drop_fns θ e {struct e} :=
+  match e with
+  | Econstr x c ys e => Econstr x c ys (drop_fns θ e)
+  | Ecase x ces => Ecase x (drop_fns_ces' drop_fns θ ces)
+  | Eproj x c n y e => Eproj x c n y (drop_fns θ e)
+  | Eletapp x f ft ys e => Eletapp x f ft ys (drop_fns θ e)
+  | Efun fds e => Efun (drop_fns_fds' drop_fns θ fds) (drop_fns θ e)
+  | Eapp f ft xs => Eapp f ft xs
+  | Eprim x p ys e => Eprim x p ys (drop_fns θ e)
+  | Ehalt x => Ehalt x
+  end.
+Definition drop_fns_ces := drop_fns_ces' drop_fns.
+Definition drop_fns_fds := drop_fns_fds' drop_fns.
+
+Ltac collapse_primes' :=
+  change (count_ces' count_exp) with count_ces in *;
+  change (count_fds' count_exp) with count_fds in *;
+  change (census_ces' census_exp) with census_ces in *;
+  change (census_fds' census_exp) with census_fds in *;
+  change (drop_fns_ces' drop_fns) with drop_fns_ces in *;
+  change (drop_fns_fds' drop_fns) with drop_fns_fds in *;
+  (* TODO: move to proto_util? *)
+  change (ces_of_proto' exp_of_proto) with ces_of_proto in *;
+  change (fundefs_of_proto' exp_of_proto) with fundefs_of_proto in *.
+
+(** * State variable *)
+
+Definition S_shrink {A} (C : exp_c A exp_univ_exp) (e : univD A) : Set := {
+  '(δ, θ) : c_map * b_map | 
+  (* The program being transformed, after all dead functions in θ have been eliminated *)
+  let P := drop_fns θ (C ⟦ e ⟧) in
+  (* The program has unique bindings only after dead functions have been dropped *)
+  unique_bindings ![P] /\
+  (* Though function bodies are copied for inlining, bound vars and free vars still disjoint
+     even before dropping dead fns *)
+  Disjoint _ (bound_var ![C ⟦ e ⟧]) (occurs_free ![C ⟦ e ⟧]) /\
+  (* δ holds valid occurrence counts *)
+  (forall x, census_count x δ = count_exp x P) /\
+  (* θ only holds dead functions *)
+  (forall f, if getd false ![f] θ then count_exp f (C ⟦ e ⟧) = 0 else True) }.
+
+Instance Preserves_S_shrink : Preserves_S _ exp_univ_exp (@S_shrink).
+Proof. constructor; intros A B fs f x δ; exact δ. Defined.
+
+Definition R_shrink : forall {A}, exp_c A exp_univ_exp -> Set := R_prod (@R_fns) (@R_ctors).
+
+(** * Delayed renaming *)
+
+(* TODO: move to proto_util *)
+Definition domain' (σ : r_map) := domain (fun x => M.get x σ).
+
+(* TODO: move to proto_util *)
+Lemma empty_domain' : domain' (M.empty _) <--> Empty_set _.
+Proof.
+  split; unfold domain', domain; [|inversion 1].
+  intros x [y Hxy]; now rewrite M.gempty in Hxy.
+Qed.
+
+Definition bound {A} : univD A -> Ensemble cps.var :=
+  match A with
+  | exp_univ_prod_ctor_tag_exp => fun '(_, e) => bound_var ![e]
+  | exp_univ_list_prod_ctor_tag_exp => fun ces => bound_var_ces ![ces]
+  | exp_univ_fundef => fun '(Ffun (mk_var x) _ xs e) => x |: FromList ![xs] :|: bound_var ![e]
+  | exp_univ_list_fundef => fun fds => bound_var_fundefs ![fds]
+  | exp_univ_exp => fun e => bound_var ![e]
+  | exp_univ_var => fun _ => Empty_set _
+  | exp_univ_fun_tag => fun _ => Empty_set _
+  | exp_univ_ctor_tag => fun _ => Empty_set _
+  | exp_univ_prim => fun _ => Empty_set _
+  | exp_univ_N => fun _ => Empty_set _
+  | exp_univ_list_var => fun _ => Empty_set _
+  end.
+
+Definition D_rename {A} (e : univD A) : Set := {
+  σ : r_map | 
+  Disjoint _ (domain' σ) (bound e) /\ 
+  Disjoint _ (image'' σ) (bound e) }.
+
+Definition rename {A} (σ : r_map) : univD A -> univD A :=
+  match A with
+  | exp_univ_prod_ctor_tag_exp => fun '(c, e) => (c, rename_all' σ e)
+  | exp_univ_list_prod_ctor_tag_exp => fun ces => map (fun '(c, e) => (c, rename_all' σ e)) ces
+  | exp_univ_fundef => fun '(Ffun f ft xs e) => Ffun f ft xs (rename_all' σ e)
+  | exp_univ_list_fundef => fun fds => map (fun '(Ffun f ft xs e) => Ffun f ft xs (rename_all' σ e)) fds
+  | exp_univ_exp => fun e => rename_all' σ e
+  | exp_univ_var => fun x => apply_r' σ x
+  | exp_univ_fun_tag => fun ft => ft
+  | exp_univ_ctor_tag => fun c => c
+  | exp_univ_prim => fun p => p
+  | exp_univ_N => fun n => n
+  | exp_univ_list_var => fun xs => apply_r_list' σ xs
+  end.
+
+(* TODO: move to proto_util *)
+Lemma apply_r'_id x : apply_r' (M.empty _) x = x.
+Proof. unbox_newtypes; unfold apply_r', apply_r; cbn; now rewrite M.gempty. Qed.
+
+Fixpoint apply_r_list'_id xs {struct xs} : apply_r_list' (M.empty _) xs = xs.
+Proof.
+  destruct xs as [|x xs]; [reflexivity|cbn].
+  change (map _ xs) with (apply_r_list' (M.empty _) xs).
+  rewrite apply_r_empty, apply_r_list'_id; now unbox_newtypes.
+Qed.
+
+(* TODO: move to proto_util *)
+Fixpoint rename_all_id e {struct e} : rename_all' (M.empty _) e = e.
+Proof.
+  destruct e; unbox_newtypes; cbn; try now rewrite ?apply_r_list'_id, ?apply_r'_id, ?rename_all_id, ?apply_r_empty.
+  Guarded.
+  - rewrite apply_r_empty; f_equal; induction ces as [|[c e] ces IHces]; [reflexivity|cbn].
+    now rewrite IHces, rename_all_id.
+  - rewrite rename_all_id; f_equal; induction fds as [|[f ft xs e_body] fds IHfds]; [reflexivity|cbn].
+    now rewrite IHfds, rename_all_id.
+Qed.
+
+Instance Delayed_D_rename : Delayed (@D_rename).
+Proof.
+  unshelve econstructor.
+  - intros A e [σ Hσ]; exact (rename σ e).
+  - intros A e; exists (M.empty _); rewrite empty_domain', empty_image; eauto with Ensembles_DB.
+  - cbn; intros; destruct A; cbn in *; unbox_newtypes;
+      repeat match goal with |- context [let '_ := ?e in _] => destruct e end;
+      rewrite ?apply_r_empty, ?apply_r'_id, ?apply_r_list'_id, ?rename_all_id; auto;
+      apply MCList.map_id_f; intros []; cbn; now rewrite rename_all_id.
+Defined.
+
+(** * Functional definition *)
+
+Fixpoint find_case (c : ctor_tag) (ces : list (ctor_tag * exp)) : option exp :=
+  match ces with
+  | [] => None
+  | (c', e) :: ces => if ![c] =? ![c'] then Some e else find_case c ces
+  end%positive.
+
+Fixpoint find_case_In c e ces : find_case c ces = Some e -> In (c, e) ces.
+Proof.
+  destruct ces as [|[c' e'] ces IHces]; [inversion 1|unbox_newtypes; cbn].
+  destruct (Pos.eqb_spec c c'); intros Heq; inv Heq; [now left|right; auto].
+Qed.
+
+Definition rw_inline' : rewriter exp_univ_exp shrink_step (@D_rename) (@R_shrink) (@S_shrink).
+Proof.
+  mk_rw; try lazymatch goal with |- ExtraVars _ -> _ => clear | |- ConstrDelay _ -> _ => clear end.
+  - (* Case folding *) intros _ R C x ces d r s success failure.
+    destruct r as [ρ1 [ρ2 Hρ]] eqn:Hr.
+    destruct d as [σ Hσ] eqn:Hd; unfold delayD, Delayed_D_rename in *.
+    pose (x0 := apply_r' σ x); specialize success with (x0 := x0).
+    destruct (M.get ![x0] ρ2) as [[c ys]|] eqn:Hctor; [|cond_failure].
+    pose (Hρ' := Hρ x0 c ys Hctor); specialize success with (c := c) (ys := ys).
+    destruct (find_case c ces) as [e|] eqn:Hfind; [|cond_failure]; apply find_case_In in Hfind.
+    specialize success with (e := e) (e0 := @rename exp_univ_exp σ e).
+    specialize success with (ces0 := @rename exp_univ_list_prod_ctor_tag_exp σ ces).
+    cond_success success; unshelve eapply success.
+    + exists σ; clear - Hfind Hσ; destruct x as [x]; cbn in *; destruct Hσ as [Hdom Hran].
+      rewrite bound_var_Ecase in *; collapse_primes'.
+      (* TODO: hoist *)
+      assert (In_ces_bound : forall c e ces, In (c, e) ces -> bound_var ![e] \subset bound_var_ces ![ces]). {
+        clear; induction ces as [|[[c'] e'] ces IHces]; [inversion 1|].
+        destruct 1 as [Heq|Hne]; [inv Heq|]; cbn; eauto with Ensembles_DB. }
+      split; (eapply Disjoint_Included_r; [eapply In_ces_bound; eauto|]; eauto).
+    + split; auto; apply in_map with (f := @rename exp_univ_prod_ctor_tag_exp σ) in Hfind; now cbn in Hfind.
+    + reflexivity. + reflexivity. + exact r.
+    + destruct s as [[δ θ] Hs] eqn:Hs_eq; unshelve eexists; [refine (_, θ)|].
+      * (* properly update counts *) admit.
+      * split; [|split; [|split]].
+        -- (* UB(θ(C[σ(Ecase x ces)])) ==> UB(θ(C[σ(e)])) because (c, e) ∈ ces *)
+           admit.
+        -- (* BV(C[σ(e)]) ⊆ BV(C[σ(Ecase x ces)]) and ditto for FV
+              And already have BV(C[σ(Ecase x es)]) # FV(C[σ(Ecase x ces)]) *)
+           admit.
+        -- admit.
+        -- destruct Hs as [Huniq [Hdis [Hδ Hθ]]].
+           (* |C[σ(e)]|f = |C|f + |σ(e)|f
+                ≤ |C|f + |σ(Ecase x ces)|f (because e ∈ ces)
+                = |C[σ(Ecase x ces)]|f
+                = 0 (by Hθ) *)
+           admit.
+  - (* Projection folding *) intros _ R C y t n x e d r s success failure.
+    destruct r as [ρ1 [ρ2 Hρ]] eqn:Hr.
+    destruct d as [σ Hσ] eqn:Hd; unfold delayD, Delayed_D_rename in *.
+    pose (x0 := apply_r' σ x); specialize success with (x0 := x0).
+    destruct (M.get ![x0] ρ2) as [[c ys]|] eqn:Hctor; [|cond_failure].
+    pose (Hρ' := Hρ x0 c ys Hctor); specialize success with (c := c) (ys := ys).
+    destruct (nthN ys n) as [y'|] eqn:Hy'; [|cond_failure].
+    specialize success with (y0 := y) (t0 := t) (n0 := n) (y' := y').
+    specialize success with (e0 := @rename exp_univ_exp σ e).
+    cond_success success; unshelve eapply success.
+    + exists σ; clear - Hσ; unbox_newtypes; cbn in *; destruct Hσ as [Hdom Hran].
+      repeat normalize_bound_var_in_ctx.
+      split; (eapply Disjoint_Included_r; [|eassumption]; eauto with Ensembles_DB).
+    + split; auto; apply in_map with (f := @rename exp_univ_prod_ctor_tag_exp σ) in Hfind; now cbn in Hfind.
+    + reflexivity. + reflexivity. + exact r.
+    + destruct s as [[δ θ] Hs] eqn:Hs_eq; unshelve eexists; [refine (_, θ)|].
+      * (* properly update counts *) admit.
+      * split; [|split; [|split]].
+        -- (* TODO: there should be a more direct proof using
+                Θ(C[σ(Eproj y t n x e)])
+                  = θ(C)[θ(σ(Eproj y t n x e))] 
+                  = θ(C)[Eproj y t n (σ(x)) (θ(σ(e)))]
+                because Hs gives UB(θ(C[σ(Eproj y t n x e)])) *)
+           (* UB(θ(C[σ(e)[y'/y]])) ⟸ UB(θ(C)) ∧ UB(θ(σ(e)[y'/y])) ∧ BV(θ(C)) # BV(θ(σ(e)[y'/y]))
+                UB(θ(C)) by assumption
+                UB(θ(σ(e)[y'/y])) ⟸ UB(θ(σ(e))) because {y', y} # BV(θ(σ(e)))
+                  y ∉ BV(θ(σ(e))) ⟸ y ∈ BV(σ(Eproj y t n x e)) ∧ UB(σ(EProj y t n x e))
+                  y' ∉ BV(θ(σ(e))) ⟸
+                    If y' ∈ BVstem(C) then y' ∈ BVstem(θ(C))
+                      (Can only drop dead variables, but y' ∈ ys and (x ↦ (c, ys)) ∈ C so y' can't be dead)
+                      ⟹ y' ∉ BV(θ(σ(e))) because UB
+                    If y' ∉ BVstem(C) then y' ∈ ys ∧ (x ↦ (c, ys)) ∈ C ⟹ y' ∈ FV(θ(C))
+                      ⟹ y' ∉ BV(θ(σ(e))) because FV(θ(C[σ(e)])) # BV(θ(C[σ(e)]))
+                BV(θ(C)) # BV(θ(σ(e)[y'/y]))
+                  ⟺ BV(θ(C)) # BV(θ(σ(e))) because {y, y'} # BV(θ(σ(e)))
+                  ⟸ BV(θ(C)) # BV(θ(σ(Eproj y t n x e)))
+                  ⟸ UB(θ(C[σ(Eproj y t n x e)])) *)
+           admit.
+        -- admit. (* TODO *)
+        -- admit. (* TODO *)
+        -- destruct Hs as [Huniq [Hdis [Hδ Hθ]]].
+           (* f ≠ y' because y' is used somewhere in C and so can't be dead
+              f ≠ y because θ contains only function bindings and y isn't a function binding
+                TODO: need to add this or some other property to θ
+              Then
+                |C[σ(e)[y'/y]]|f = |C|f + |σ(e)[y'/y]|f
+                  = |C|f + |σ(e)|f (because f ∉ {y, y'})
+                  ≤ |C|f + |σ(Eproj y t n x e)|f
+                  = |C[σ(Eproj y t n x e)]|f
+                  = 0 (by Hθ) *)
+           admit.
+  - (* Top down dead constr *) intros _ R C x c ys e d r s success failure.
+    destruct s as [[δ θ] [Huniq [Hdis [Hδ Hθ]]]] eqn:Hs, d as [σ Hσ] eqn:Hd; unfold delayD, Delayed_D_rename in *.
+    destruct (M.get ![x] δ) eqn:Hcount; [cond_failure|].
+    specialize success with (x0 := x) (c0 := c) (ys0 := apply_r_list' σ ys).
+    specialize success with (e0 := @rename exp_univ_exp σ e); cond_success success; unshelve eapply success.
+    + exists σ. admit. (* easy *)
+    + (* δ(x) = |θ(C[σ(Econstr x c ys e)])|x = 0
+         TODO: Hδ isn't strong enough: what if x occurs free in one of the dropped functions?
+           This seems tricky to fix. *)
+      admit.
+    + reflexivity. + reflexivity. + exact r.
+    + unshelve eexists; [refine (_, θ)|].
+      * (* update counts properly *)
+        admit.
+      * split; [|split; [|split]].
+        -- (* Follows from Huniq because θ(C[σ(Econstr x c ys e)]) = θ(C)[Econstr x c (σ(ys)) (θ(σ(e)))] *)
+           admit.
+    pose (x0 := apply_r' σ x); specialize success with (x0 := x0).
+    admit.
+  - (* Bottom up dead constr *) intros _ R C x c ys e r s success failure.
+    admit.
+  - (* Top down dead proj *) intros _ R C x t n y e d r s success failure.
+    admit.
+  - (* Bottom up dead proj *) intros _ R C x t n y e r s success failure.
+    admit.
+  - (* Top down dead prim *) intros _ R C x p ys e d r s success failure.
+    admit.
+  - (* Bottom up dead prim *) intros _ R C x p ys e r s success failure.
+    admit.
+  - (* Top down dead fun *) intros _ R C f ft xs e fds d r s success failure.
+    admit.
+  - (* Bottom up dead fun *) intros _ R C f ft xs e fds r s success failure.
+    admit.
+  - (* Top down dead bundle *) intros _ R C e r s success failure.
+    admit.
+  - (* Shrink inlining (CPS) *) intros _ R C f ft ys d r s success failure.
+    admit.
+  - (* Rename a pair *) intros _ R c e d k.
+    admit.
+  - (* Rename empty list *) intros _ R d k.
+    admit.
+  - (* Rename cons case arms *) intros _ R [c e] ces d k.
+    admit.
+  - (* Rename function definition *) intros _ R f ft xs e d k.
+    admit.
+  - (* Rename empty list *) intros _ R d k.
+    admit.
+  - (* Rename cons function definitions *) intros _ R fd fds d k.
+    admit.
+  - (* Rename constr binding *) intros _ R x c ys e d k.
+    admit.
+  - (* Rename case expression *) intros _ R x ces d k.
+    admit.
+  - (* Rename proj binding *) intros _ R x t n y e d k.
+    admit.
+  - (* Rename letapp *) intros _ R x f ft ys e d k.
+    admit.
+  - (* Rename bundle definition *) intros _ R fds e d k.
+    admit.
+  - (* Rename cps app *) intros _ R f ft ys d k.
+    admit.
+  - (* Rename prim binding *) intros _ R x p ys e d k.
+    admit.
+  - (* Rename halt *) intros _ R x d k.
+    admit.
+  - (* Fuse renaming for proj folding *) destruct d0 as [σ Hσ] eqn:Hσ_eq; rewrite <- Hσ_eq in *.
+    unshelve eexists; [exists (M.set ![y] ![y'] σ)|unbox_newtypes; cbn; subst d0].
+    + admit.
+    + admit.
+  - (* Fuse renaming for inlining *) destruct d0 as [σ' Hσ'] eqn:Hσ'_eq; rewrite <- Hσ'_eq in *.
+    destruct (set_lists ![xs] ![ys] σ') as [σ''|] eqn:Hσ''.
+    2: { exfalso. apply set_lists_length_eq in H25.
+         apply set_lists_length3 with (rho := σ') in H25.
+         destruct H25 as [σ'' Hσ''']; congruence. }
+    unshelve eexists; [exists σ''|unbox_newtypes; cbn; subst d0].
+    + admit.
+    + admit.
+Admitted.
